src/FcEtt/toplevel.v
@@ -26,21 +26,27 @@ Proof.
 Qed.
 
 (* ------------------------------------------ *)
-Lemma toplevel_closed : forall F a A, binds F (Ax a A) toplevel ->
-                                 Typing nil a A.
+Lemma toplevel_closed : forall F a A R, binds F (Ax a A R) toplevel ->
+                                 Typing nil a A R.
 Proof.
   have st: Sig toplevel by apply Sig_toplevel.
   induction st.
   - intros. inversion H.
-  - intros. inversion H2. inversion H3. subst. eauto. eauto.
+  - intros.
+    match goal with [ H : binds ?F _ _ |- _ ] => inversion H end.
+    match goal with [ H : (_,_) = (_,_) |- _ ] => inversion H end.
+    subst. eauto. eauto.
 Qed.
 
 
-Lemma an_toplevel_closed : forall F a A, binds F (Ax a A) an_toplevel ->
-                                    AnnTyping nil a A.
+Lemma an_toplevel_closed : forall F a A R, binds F (Ax a A R) an_toplevel ->
+                                    AnnTyping nil a A R.
 Proof.
   have st: AnnSig an_toplevel by apply AnnSig_an_toplevel.
   induction st.
   - intros. inversion H.
-  - intros. inversion H2. inversion H3. subst. eauto. eauto.
+  - intros.
+    match goal with [ H : binds ?F _ _ |- _ ] => inversion H end.
+    match goal with [ H : (_,_) = (_,_) |- _ ] => inversion H end.
+    subst. eauto. eauto.
 Qed.
